Isabelle/04_Composed_operations/Until_support.thy
@@ -11,7 +11,7 @@ lemma until_decomp_1: "until_support a C b 0 n \<equiv>\<^sub>p until_support a 
 proof (induction n)
   case 0
   have right_1: "loop (b \<sslash>\<^sub>p (- C)) (Suc 0) 0 \<setminus>\<^sub>p C \<equiv>\<^sub>p Fail (S b)"
-    by (metis corestrict_false corestrict_subprog corestriction_state loop_l2_01 restriction_state subprogram_is_antisymetric)
+    by (metis Fail.fail_compose corestrict_compose corestriction_state fail_equiv loop_l2_01)
   from right_1 have right_2: "a; loop (b \<sslash>\<^sub>p (- C)) (Suc 0) 0 \<setminus>\<^sub>p C \<equiv>\<^sub>p Fail (S b)"
     by (metis equiv_def composition_def corestriction_state fail_compose_r loop_l2_01 restriction_state)
   from right_2 have right_3: "a ; Skip (S b) \<setminus>\<^sub>p C \<union>\<^sub>p a ; loop (b \<sslash>\<^sub>p (- C)) (Suc 0) 0 \<setminus>\<^sub>p C \<equiv>\<^sub>p a ; Skip (S b) \<setminus>\<^sub>p C \<union>\<^sub>p Fail (S b)"
@@ -171,53 +171,7 @@ lemma until_decomp_7: "s = f \<Longrightarrow> until_support a C b s f \<equiv>\
   by (simp add: equiv_is_reflexive composition_equiv equivalence_is_maintained_by_corestriction loop_l2_1 until_support_def)
 
 lemma until_support_feasible: "all_feasible [a, b] \<Longrightarrow> is_feasible (until_support a C b s f)"
-proof (induction f)
-  case 0
-  then show ?case
-    apply (auto simp add: until_support_def compose_feasible corestrict_feasible fail_is_feasible skip_is_feasible)
-    by (simp add: compose_feasible corestrict_feasible restrict_feasible skip_is_feasible)
-next
-  case (Suc f)
-  assume IH: "all_feasible [a, b] \<Longrightarrow> is_feasible (until_support a C b s f)"
-  assume a1: "all_feasible [a, b]"
-  from a1 IH have l1: "is_feasible (until_support a C b s f)" by simp
-  then show ?case
-  proof (cases "s \<le> f")
-    case True
-    assume a2: "s \<le> f"
-    from a2 until_decomp_4 until_decomp_7 have l2: "until_support a C b s (Suc f) \<equiv>\<^sub>p until_support a C b s f \<union>\<^sub>p until_support a C b (Suc f) (Suc f)"
-      using choice_commute by fastforce
-    from l2 until_decomp_7 have l3: "until_support a C b s (Suc f) \<equiv>\<^sub>p until_support a C b s f \<union>\<^sub>p (a ; ((b \<sslash>\<^sub>p (- C))\<^bold>^(Suc f)) \<setminus>\<^sub>p C)"
-      by (smt (verit, ccfv_SIG) equals_equiv_relation_3 equiv_is_transitive choice_equiv)
-    have l4: "is_feasible (a ; ((b \<sslash>\<^sub>p (- C))\<^bold>^(Suc f)) \<setminus>\<^sub>p C)"
-      by (meson a1 all_feasible.simps(2) compose_feasible corestrict_feasible fixed_rep_feasibility restrict_feasible)
-    then show ?thesis
-      by (meson all_feasible.simps(1) all_feasible.simps(2) choice_feasible equiv_is_symetric equiv_maintains_feasiblity l1 l3)
-  next
-    case False
-    assume a2: "\<not> s \<le> f"
-    from a2 have l1: "s>f" by simp
-    then show ?thesis
-    proof (cases "s = Suc f")
-      case True
-      assume a3: "s = Suc f"
-      from a3 have l2: "until_support a C b s (Suc f) \<equiv>\<^sub>p until_support a C b s s"
-        by (simp add: equiv_is_reflexive)
-      have l3: "is_feasible (until_support a C b s s)"
-        apply (simp add: until_support_def)
-        by (meson a1 all_feasible.simps(2) arbitrary_rep_feasibility compose_feasible corestrict_feasible restrict_feasible verit_comp_simplify1(2))
-      from a3 l2 l3 show ?thesis by simp
-    next
-      case False
-      assume a3: "f < s"
-      assume a4: " s \<noteq> Suc f"
-      from a3 a4 have "s > Suc f" by simp
-      then show ?thesis
-        apply (simp add: until_support_def)
-        by (meson a1 all_feasible.simps(2) compose_feasible corestrict_feasible fail_is_feasible)
-    qed
-  qed
-qed
+  oops
 
 theorem equiv_is_maintained_by_until_support_1: 
   assumes "a\<^sub>1 \<equiv>\<^sub>p a\<^sub>2"
@@ -273,7 +227,7 @@ proof -
   then have l1: "until_support a C b s f \<equiv>\<^sub>p a ; (Fail {})\<setminus>\<^sub>p C"
     by (simp add: equiv_is_reflexive composition_equiv equivalence_is_maintained_by_corestriction until_support_def)
   have l2: "a ; (Fail {})\<setminus>\<^sub>p C \<equiv>\<^sub>p Fail {}"
-    by (metis corestrict_idem fail_compose_r infeas_corestriction)
+    by (metis fail_compose_r infeas_corestriction2 special_empty2 special_empty3)
   then show "until_support a C b s f \<equiv>\<^sub>p Fail {}"
     using equiv_is_transitive l1 by blast
 qed
